Renamed chapters 06 and 08 to midterm-project and final-project

chapter06/exercises/exercise01.dfy
@@ -1,38 +1,465 @@
-//Your goal is to build a distributed lock server. This challenge differs from
-//LockServer in two ways. First, there is no central server that coordinates
-//the activity. Second, the hosts can communicate only via asynchronous
-//messages; a single state machine transition cannot simultaneously read or
-//update the state of two hosts.
-//
-//To guard against duplicate messages, the nodes associate a monotonically
-//increasing epoch number with the lock. Initially, node 0 holds the lock and
-//its epoch number is 1. A node that holds the lock can “grant” it to another
-//node by sending them a “Grant” message which has an epoch number that is
-//greater than the node’v epoch number. A node that receives such a message
-//will become the new holder and will set its epoch number to the message’v
-//epoch number.
+include "../../library/library.dfy"
 
-// You'll first need to modify 'protocol.i.dfy' to define the protocol message
-// format and the host behavior.
-// Then come back here define the safety condition and prove that the
-// distributed system made from that protocol maintains it.
+module Types {
+  // TODO finite domain of keys so we can use finite-domained maps and avoid manager nonsense
+  type Key(==, !new)
 
-include "distributed_system.s.dfy"
+  // Assume a finite domain (set is finite) of possible keys, so we
+  // can use (finite) maps. Dafny also offers infinite maps, but those
+  // bring another twist, so let's just use what's familiar for now.
+  function AllKeys() : set<Key>
 
-// Replace 'false' with an appropriate safety condition: no two clients hold
-// the lock simulatneously.
-predicate Safety(v:DistVars) {
-  false
+  type Value(==, !new)
+    // (==) means whatever this type is, it has equality defined on it.
+    // !new means this type can't be allocated on the heap; it's a mathematical
+    // immutable object.
+    // Since we're in math-land, not implementation-land, we always want both features
+    // of all types, so we declare them on these otherwise-unspecified types.
+    // Missing == gives "map domain type must support equality" errors.
+    // Missing !new gives "...not allowed to depend on the set of allocated references" errors.
+
+  function DefaultValue() : Value
+    // No body -> this is an axiom.
+
+  function InitialMap() : map<Key, Value>
+  {
+    map key | key in AllKeys() :: DefaultValue()
+  }
 }
 
-// Replace 'true' with an invariant that's induction and supports Safety.
-predicate Inv(v:DistVars) {
-  true
+module MapSpec {
+  import opened Types
+
+  datatype Variables = Variables(mapp:map<Key, Value>)
+
+  predicate Init(v: Variables)
+  {
+    v.mapp == InitialMap()
+  }
+
+  predicate InsertOp(v:Variables, v':Variables, key:Key, value:Value)
+  {
+    && key in AllKeys()
+    && v'.mapp == v.mapp[key := value]
+  }
+
+  predicate QueryOp(v:Variables, v':Variables, key:Key, output:Value)
+  {
+    && key in AllKeys()
+    && (output == if key in v.mapp then v.mapp[key] else DefaultValue())
+    && v' == v  // no change to map state
+  }
+
+  datatype Step =
+    | InsertOpStep(key:Key, value:Value)
+    | QueryOpStep(key:Key, output:Value)
+    | NoOpStep()
+
+  predicate NextStep(v: Variables, v': Variables, step:Step)
+  {
+    match step
+      case InsertOpStep(key, value) => InsertOp(v, v', key, value)
+      case QueryOpStep(key, output) => QueryOp(v, v', key, output)
+      case NoOpStep => v' == v
+  }
+
+  predicate Next(v: Variables, v': Variables)
+  {
+    exists step :: NextStep(v, v', step)
+  }
 }
 
-lemma SafetyProof()
-  ensures forall v :: DistInit(v) ==> Inv(v)
-  ensures forall v, v' :: Inv(v) && DistNext(v, v') ==> Inv(v')
-  ensures forall v :: Inv(v) ==> Safety(v)
-{
+// A "synchronous" KV store (network messages are delivered
+// instantaneously).
+
+module Implementation {
+  import opened Types
+
+  type HostIdx = nat
+
+  datatype Constants = Constants(mapCount: nat)
+  {
+    predicate WF() { 0 < mapCount }
+    predicate ValidHost(idx: HostIdx) { idx < mapCount }
+  }
+
+  datatype Variables = Variables(maps:seq<map<Key, Value>>)
+  {
+    predicate WF(c: Constants) { |maps| == c.mapCount }
+  }
+
+  predicate Init(c: Constants, v: Variables)
+  {
+    && v.WF(c)
+    && (forall idx:HostIdx | c.ValidHost(idx) :: v.maps[idx] == if idx==0 then InitialMap() else map[])
+  }
+
+  predicate Insert(c: Constants, v: Variables, v': Variables, idx: HostIdx, key: Key, value: Value)
+  {
+    && v.WF(c)
+    && c.ValidHost(idx)
+    && key in v.maps[idx] // the participating "host" needs to be authoritative on this key
+    //&& key in AllKeys() // implied by previous conjunct + Inv()ariant
+    && v'.maps == v.maps[idx := v.maps[idx][key := value]]
+  }
+
+  predicate Query(c: Constants, v: Variables, v': Variables, idx: HostIdx, key: Key, output: Value)
+  {
+    && v.WF(c)
+    && c.ValidHost(idx)
+    && key in v.maps[idx] // the participating "host" needs to be authoritative on this key
+    && output == v.maps[idx][key]
+    && v' == v  // UNCHANGED
+  }
+
+  function {:opaque} MapRemoveOne<K,V>(m:map<K,V>, key:K) : (m':map<K,V>)
+    ensures forall k :: k in m && k != key ==> k in m'
+    ensures forall k :: k in m' ==> k in m && k != key
+    ensures forall j :: j in m' ==> m'[j] == m[j]
+    ensures |m'.Keys| <= |m.Keys|
+    ensures |m'| <= |m|
+  {
+    var m':= map j | j in m && j != key :: m[j];
+    assert m'.Keys == m.Keys - {key};
+    m'
+  }
+
+  // A possible enhancement exercise: transfer many key,value pairs in one step
+  predicate Transfer(c: Constants, v: Variables, v': Variables, sendIdx: HostIdx, recvIdx: HostIdx, key: Key, value: Value)
+  {
+    && v.WF(c)
+    && v'.WF(c)
+    && c.ValidHost(sendIdx)
+    && c.ValidHost(recvIdx)
+    && key in v.maps[sendIdx]
+    && v.maps[sendIdx][key] == value
+    && v'.maps[sendIdx] == MapRemoveOne(v.maps[sendIdx], key)  // key leaves sending map
+    && v'.maps[recvIdx] == v.maps[recvIdx][key := value]    // key appears in recv map
+    && (forall otherIdx:HostIdx | c.ValidHost(otherIdx) && otherIdx != sendIdx && otherIdx != recvIdx
+        :: v'.maps[otherIdx] == v.maps[otherIdx]) // unchanged other participants
+  }
+
+  datatype Step =
+    | InsertStep(idx: HostIdx, key: Key, value: Value)
+    | QueryStep(idx: HostIdx, key: Key, output: Value)
+    | TransferStep(sendIdx: HostIdx, recvIdx: HostIdx, key: Key, value: Value)
+
+  predicate NextStep(c: Constants, v: Variables, v': Variables, step: Step)
+  {
+    match step
+      case InsertStep(idx, key, value) => Insert(c, v, v', idx, key, value)
+      case QueryStep(idx, key, output) => Query(c, v, v', idx, key, output)
+      case TransferStep(sendIdx, recvIdx, key, value) => Transfer(c, v, v', sendIdx, recvIdx, key, value)
+  }
+
+  predicate Next(c: Constants, v: Variables, v': Variables)
+  {
+    exists step :: NextStep(c, v, v', step)
+  }
+}
+
+module RefinementProof {
+  import opened Library
+  import opened Types
+  import MapSpec
+  import opened Implementation
+
+  predicate HostHasKey(c: Constants, v: Variables, hostidx:HostIdx, key:Key)
+    requires v.WF(c)
+  {
+    && c.ValidHost(hostidx)
+    && key in v.maps[hostidx]
+  }
+
+  // Pulling the choose out into its own function is sometimes necessary due
+  // to a (deliberate) stupidity in Dafny: it doesn't treat :| expressions
+  // as subsitution-equivalent, even though the are (as evidenced by pulling
+  // one into a function).
+  function TheHostWithKey(c: Constants, v: Variables, key:Key) : HostIdx
+    requires v.WF(c)
+    requires exists hostidx :: HostHasKey(c, v, hostidx, key);
+  {
+    var hostidx:HostIdx :| HostHasKey(c, v, hostidx, key);
+    hostidx
+  }
+
+
+  function AbstractionOneKey(c: Constants, v: Variables, key:Key) : Value
+    requires v.WF(c)
+  {
+    if exists idx :: HostHasKey(c, v, idx, key)
+    then
+      v.maps[TheHostWithKey(c, v, key)][key]
+    else DefaultValue()
+  }
+
+  // We construct the finite set of possible map keys here, all
+  // because we need to supply Dafny with simple evidence that our map domain
+  // is finite for the map comprehension in Abstraction().
+  // (An alternative would be to switch to imaps -- maps with potentially-infinite
+  // domains -- but that would require making the spec fancier. This was a compromise.)
+
+  // The sequence of map domains. Pulled out into its own function to
+  // make proof assertions easy to write.
+  function MapDomains(c: Constants, v: Variables) : seq<set<Key>>
+    requires v.WF(c)
+  {
+    seq(c.mapCount, i requires 0<=i<c.mapCount => v.maps[i].Keys)
+  }
+
+  function KnownKeys(c: Constants, v: Variables) : set<Key>
+    requires v.WF(c)
+  {
+    UnionSeqOfSets(MapDomains(c, v))
+  }
+
+  // Packaged as lemma. Proves trivially as ensures of KnownKeys,
+  // but creates a trigger storm.
+  lemma HostKeysSubsetOfKnownKeys(c: Constants, v: Variables, count: nat)
+    requires v.WF(c)
+    requires count <= c.mapCount
+    ensures forall idx | 0 <= idx < count :: v.maps[idx].Keys <= KnownKeys(c, v)
+  {
+    forall idx | 0 <= idx < count ensures v.maps[idx].Keys <= KnownKeys(c, v)
+    {
+      SetsAreSubsetsOfUnion(MapDomains(c, v));
+      assert v.maps[idx].Keys == MapDomains(c, v)[idx];  // trigger
+    }
+  }
+
+  function Abstraction(c: Constants, v: Variables) : MapSpec.Variables
+    requires v.WF(c)
+  {
+    MapSpec.Variables(map key | key in KnownKeys(c, v) :: AbstractionOneKey(c, v, key))
+  }
+
+  // This does slow things down quite a bit.
+  predicate {:opaque} KeysHeldUniquely(c: Constants, v: Variables)
+    requires v.WF(c)
+  {
+    forall key, hostidx:HostIdx, otherhost:HostIdx
+        | && c.ValidHost(hostidx) && c.ValidHost(otherhost)
+          && key in v.maps[hostidx] && key in v.maps[otherhost]
+        :: hostidx == otherhost
+  }
+
+  predicate Inv(c: Constants, v: Variables)
+  {
+    && v.WF(c)
+    // Every key lives somewhere.
+    && KnownKeys(c, v) == Types.AllKeys()
+    // No key lives in two places.
+    && KeysHeldUniquely(c, v)
+  }
+
+  lemma InitAllKeysEmpty(c: Constants, v: Variables, count: nat)
+    requires Init(c, v)
+    requires 0 < count <= c.mapCount
+    ensures KnownKeys(c, v) == AllKeys()
+  {
+    EachUnionMemberBelongsToASet(MapDomains(c, v));
+    SetsAreSubsetsOfUnion(MapDomains(c, v));
+    forall key | key in AllKeys() ensures key in KnownKeys(c, v) {
+      assert key in MapDomains(c,v)[0]; // trigger
+    }
+  }
+
+  lemma AllKeysMembership(c: Constants, v: Variables)
+    requires Inv(c, v)
+    ensures forall key ::
+      (key in KnownKeys(c, v) <==> exists hostidx:HostIdx :: hostidx<c.mapCount && key in v.maps[hostidx])
+  {
+    var count := c.mapCount;
+    forall key
+      | key in KnownKeys(c, v)
+      ensures exists hostidx:HostIdx :: hostidx<count && key in v.maps[hostidx]
+    {
+      EachUnionMemberBelongsToASet(MapDomains(c, v));
+      var idx :| 0<=idx<|MapDomains(c, v)| && key in MapDomains(c, v)[idx];
+      assert count == |MapDomains(c, v)|;
+      assert v.maps[idx].Keys == MapDomains(c,v)[idx];
+      assert idx<count && key in v.maps[idx]; // trigger
+    }
+    forall key
+      | exists hostidx:HostIdx :: hostidx<count && key in v.maps[hostidx]
+      ensures key in KnownKeys(c, v)
+    {
+      var hostidx:HostIdx :| hostidx<count && key in v.maps[hostidx];
+      SetsAreSubsetsOfUnion(MapDomains(c, v));
+      assert key in MapDomains(c, v)[hostidx];
+      assert MapDomains(c, v)[hostidx] <= KnownKeys(c, v);
+      assert key in KnownKeys(c, v);
+    }
+  }
+
+  lemma InitRefines(c: Constants, v: Variables)
+    requires c.WF()
+    requires Init(c, v)
+    ensures MapSpec.Init(Abstraction(c, v))
+    ensures Inv(c, v)
+  {
+    InitAllKeysEmpty(c, v, c.mapCount);
+    reveal_KeysHeldUniquely();
+  }
+
+  lemma ThisIsTheHost(c: Constants, v: Variables, hostidx:HostIdx, key:Key)
+    requires v.WF(c)
+    requires KeysHeldUniquely(c, v)
+    requires HostHasKey(c, v, hostidx, key)
+    ensures TheHostWithKey(c, v, key) == hostidx
+  {
+    reveal_KeysHeldUniquely();
+  }
+
+  lemma InsertPreservesInvAndRefines(c: Constants, v: Variables, v': Variables, insertHost: HostIdx, insertedKey: Key, value: Value)
+    requires Inv(c, v)
+    requires Next(c, v, v')
+    requires c.ValidHost(insertHost)
+    requires Insert(c, v, v', insertHost, insertedKey, value)
+    ensures Inv(c, v')
+    ensures MapSpec.Next(Abstraction(c, v), Abstraction(c, v'))
+  {
+    var abstractMap := Abstraction(c, v).mapp;
+    var abstractMap' := Abstraction(c, v').mapp;
+
+    assert insertedKey in AllKeys() by {
+      SetsAreSubsetsOfUnion(MapDomains(c, v));
+      assert MapDomains(c, v)[insertHost] == v.maps[insertHost].Keys; //trigger
+    }
+
+    assert KeysHeldUniquely(c, v') by { reveal_KeysHeldUniquely(); }
+
+    forall key
+      ensures key in abstractMap' <==> key in abstractMap || key == insertedKey // domain
+      ensures key in abstractMap' ==> (abstractMap'[key] == if key==insertedKey then value else abstractMap[key])  // value
+    {
+      if key == insertedKey {
+        SetsAreSubsetsOfUnion(MapDomains(c, v'));
+        assert MapDomains(c, v')[insertHost] <= KnownKeys(c, v'); // trigger
+        assert key in abstractMap'; // case goal
+      }
+      if key in abstractMap {
+        var idx := GetIndexForMember(MapDomains(c, v), key);
+        assert MapDomains(c, v')[idx] <= KnownKeys(c, v') by {
+          // The lemma below is a trigger-trap danger (causes timeouts), so I'm
+          // careful to only call it tucked way into this by clause.
+          SetsAreSubsetsOfUnion(MapDomains(c, v'));
+        }
+        assert key in abstractMap'; // case goal
+      }
+      if key in abstractMap' {
+        if key == insertedKey {
+          ThisIsTheHost(c, v', insertHost, key);
+          assert abstractMap'[key] == value;  // case goal
+        } else {
+          var keyIdx := GetIndexForMember(MapDomains(c, v'), key);
+          ThisIsTheHost(c, v', keyIdx, key);
+          ThisIsTheHost(c, v, keyIdx, key);
+          assert key in abstractMap by {
+            SetsAreSubsetsOfUnion(MapDomains(c, v));
+            assert MapDomains(c, v)[keyIdx] <= KnownKeys(c, v);  // trigger
+          }
+          assert abstractMap'[key] == abstractMap[key]; // case goal
+        }
+      }
+    }
+
+    assert KnownKeys(c, v') == Types.AllKeys() by {
+      assert abstractMap'.Keys == KnownKeys(c, v'); // trigger
+    }
+    assert MapSpec.NextStep(Abstraction(c, v), Abstraction(c, v'), MapSpec.InsertOpStep(insertedKey, value)); // witness
+  }
+
+  lemma TransferPreservesInvAndRefines(c: Constants, v: Variables, v': Variables, sendIdx: HostIdx, recvIdx: HostIdx, sentKey: Key, value: Value)
+    requires Inv(c, v)
+    requires Next(c, v, v')
+    requires c.ValidHost(sendIdx)
+    requires c.ValidHost(recvIdx)
+    requires Transfer(c, v, v', sendIdx, recvIdx, sentKey, value)
+    ensures Inv(c, v')
+    ensures MapSpec.Next(Abstraction(c, v), Abstraction(c, v'))
+  {
+    // domain preserved
+    forall key
+      ensures key in Abstraction(c, v).mapp <==> key in Abstraction(c, v').mapp
+    {
+      var idx;
+      if key in Abstraction(c, v).mapp {
+        SetsAreSubsetsOfUnion(MapDomains(c, v'));
+        if key==sentKey {
+          idx := recvIdx;
+        }
+        else {
+          idx := GetIndexForMember(MapDomains(c, v), key);
+        }
+        assert MapDomains(c, v')[idx] <= KnownKeys(c, v');  // trigger
+        assert key in Abstraction(c, v').mapp;  // case goal
+      }
+      if key in Abstraction(c, v').mapp {
+        SetsAreSubsetsOfUnion(MapDomains(c, v));
+        if key==sentKey {
+          idx := sendIdx;
+        }
+        else {
+          idx := GetIndexForMember(MapDomains(c, v'), key);
+        }
+        assert MapDomains(c, v)[idx] <= KnownKeys(c, v);  // trigger
+        assert key in Abstraction(c, v).mapp;  // case goal
+      }
+    }
+
+    assert KeysHeldUniquely(c, v') by { reveal_KeysHeldUniquely(); }
+
+    // values preserved
+    forall key | key in Abstraction(c, v).mapp
+      ensures Abstraction(c, v).mapp[key] == Abstraction(c, v').mapp[key]
+    {
+      // identify where to find key in the old & new worlds
+      var idx, idx';
+      if key == sentKey {
+        idx := sendIdx;
+        idx' := recvIdx;
+      } else {
+        idx := GetIndexForMember(MapDomains(c, v), key);
+        idx' := idx;
+      }
+//      assert v'.maps[idx'][key] == v.maps[idx][key];  // hey look same values
+
+      // Tie from particular map up to abstraction
+      ThisIsTheHost(c, v', idx', key);
+      ThisIsTheHost(c, v, idx, key);
+    }
+
+    assert KnownKeys(c, v') == Types.AllKeys() by {
+      assert KnownKeys(c, v') == Abstraction(c, v').mapp.Keys;  // trigger
+      assert KnownKeys(c, v) == Abstraction(c, v).mapp.Keys;    // trigger
+    }
+    assert MapSpec.NextStep(Abstraction(c, v), Abstraction(c, v'), MapSpec.NoOpStep); // witness
+  }
+
+  lemma NextPreservesInvAndRefines(c: Constants, v: Variables, v': Variables)
+    requires Inv(c, v)
+    requires Next(c, v, v')
+    ensures Inv(c, v')
+    ensures MapSpec.Next(Abstraction(c, v), Abstraction(c, v'))
+  {
+    var step :| NextStep(c, v, v', step);
+    match step
+      case InsertStep(idx, key, value) => {
+        InsertPreservesInvAndRefines(c, v, v', idx, key, value);
+      }
+      case QueryStep(idx, key, output) => {
+        assert v == v'; // weirdly obvious trigger
+        assert Inv(c, v') by { reveal_KeysHeldUniquely(); }
+        assert key in KnownKeys(c, v) by { HostKeysSubsetOfKnownKeys(c, v, c.mapCount); }
+        assert output == Abstraction(c, v).mapp[key] by {
+          assert HostHasKey(c, v, idx, key);  // witness
+          reveal_KeysHeldUniquely();
+        }
+        assert MapSpec.NextStep(Abstraction(c, v), Abstraction(c, v'), MapSpec.QueryOpStep(key, output)); // witness
+      }
+      case TransferStep(sendIdx, recvIdx, key, value) => {
+        TransferPreservesInvAndRefines(c, v, v', sendIdx, recvIdx, key, value);
+      }
+  }
 }
