midterm-project/exercises/exercise01.dfy
@@ -1,0 +1,38 @@
+//Your goal is to build a distributed lock server. This challenge differs from
+//LockServer in two ways. First, there is no central server that coordinates
+//the activity. Second, the hosts can communicate only via asynchronous
+//messages; a single state machine transition cannot simultaneously read or
+//update the state of two hosts.
+//
+//To guard against duplicate messages, the nodes associate a monotonically
+//increasing epoch number with the lock. Initially, node 0 holds the lock and
+//its epoch number is 1. A node that holds the lock can “grant” it to another
+//node by sending them a “Grant” message which has an epoch number that is
+//greater than the node’v epoch number. A node that receives such a message
+//will become the new holder and will set its epoch number to the message’v
+//epoch number.
+
+// You'll first need to modify 'protocol.i.dfy' to define the protocol message
+// format and the host behavior.
+// Then come back here define the safety condition and prove that the
+// distributed system made from that protocol maintains it.
+
+include "distributed_system.s.dfy"
+
+// Replace 'false' with an appropriate safety condition: no two clients hold
+// the lock simulatneously.
+predicate Safety(v:DistVars) {
+  false
+}
+
+// Replace 'true' with an invariant that's induction and supports Safety.
+predicate Inv(v:DistVars) {
+  true
+}
+
+lemma SafetyProof()
+  ensures forall v :: DistInit(v) ==> Inv(v)
+  ensures forall v, v' :: Inv(v) && DistNext(v, v') ==> Inv(v')
+  ensures forall v :: Inv(v) ==> Safety(v)
+{
+}
